src/program_proof/asyncfile/proof.v
@@ -1,0 +1,26 @@
+From Perennial.program_proof Require Import grove_prelude.
+From Goose.github_com.mit_pdos.gokv Require asyncfile.
+
+Section asyncfile_proof.
+
+Context `{!heapGS Σ}.
+Definition own_AsyncFile (N:namespace) (f:loc) (P: list u8 → iProp Σ) (data:list u8) : iProp Σ.
+Admitted.
+
+Lemma wp_AsyncFile__Write N f P olddata data_sl data Q:
+  {{{
+        "Hf" ∷ own_AsyncFile N f P olddata ∗
+        "Hdata" ∷ own_slice_small data_sl byteT 1 data ∗
+        "Hupd" ∷ (P olddata ={⊤∖↑N}=∗ P data ∗ Q)
+  }}}
+    asyncfile.AsyncFile__Write #f (slice_val data_sl)
+  {{{
+        (w:val), RET w;
+        own_AsyncFile N f P data ∗
+        WP w #() {{ _, Q }}
+  }}}
+.
+Proof.
+Admitted.
+
+End asyncfile_proof.
