src/program_proof/mpaxos/withlock_proof.v
@@ -1,0 +1,72 @@
+From Perennial.program_proof Require Import grove_prelude.
+From Goose.github_com.mit_pdos.gokv Require mpaxos.
+From Perennial.program_proof.mpaxos Require Export definitions.
+
+Section withlock_proof.
+
+Context `{!heapGS Σ}.
+
+Context `{!mpG Σ}.
+Context `{HconfigTC:!configTC}.
+
+Lemma wp_Server__withLock (s:loc) γ γsrv (f:val) Φ :
+  is_Server s γ γsrv -∗
+  (∀ ps pst,
+  paxosState.own_vol ps pst -∗
+  WP f #ps {{ λ _, ∃ pst', paxosState.own_vol ps pst' ∗
+                   (paxosState.own_ghost γ γsrv pst ={⊤∖↑fileN}=∗
+                    paxosState.own_ghost γ γsrv pst' ∗ Φ #())
+    }}) -∗
+  WP Server__withLock #s f {{ Φ }}
+.
+Proof.
+  iIntros "#Hsrv Hwp".
+  wp_lam.
+  wp_pures.
+  iNamed "Hsrv".
+  wp_loadField.
+  wp_apply (acquire_spec with "[$]").
+  iIntros "[Hlocked Hown]".
+  iNamed "Hown".
+  wp_pures.
+  wp_loadField.
+  wp_bind (f #ps).
+  wp_apply (wp_wand with "[Hwp Hvol]").
+  { wp_apply ("Hwp" with "Hvol"). }
+  iIntros (?) "Hpost".
+  iDestruct "Hpost" as (?) "[Hvol Hupd]".
+  wp_pures.
+  wp_loadField.
+  wp_apply (paxosState.wp_encode with "[$]").
+  iIntros (?) "[Hvol Hsl]".
+  wp_loadField.
+  iDestruct (own_slice_to_small with "Hsl") as "Hsl".
+  wp_apply (wp_AsyncFile__Write with "[$Hfile $Hsl Hupd]").
+  {
+    iIntros "Hi".
+    iNamed "Hi".
+    eapply inj in Henc; last apply _.
+    subst.
+    iMod ("Hupd" with "[$]") as "[Hghost HΦ]".
+    iModIntro.
+    iSplitR "HΦ".
+    { repeat iExists _; iFrame. done. }
+    iAccu.
+  }
+  iIntros (?) "[Hfile Hwp]".
+  wp_pures.
+  wp_loadField.
+  wp_apply (release_spec with "[-Hwp]").
+  {
+    iFrame "HmuInv Hlocked".
+    iNext.
+    repeat iExists _.
+    iFrame.
+  }
+  wp_pures.
+  wp_apply (wp_wand with "Hwp").
+  iIntros (?) "HΦ".
+  wp_pures. iModIntro. iFrame.
+Qed.
+
+End withlock_proof.
